add more tests

execution/tests/EscrowTests/EscrowTests.v
@@ -53,6 +53,13 @@ Module MG := EscrowGens.EscrowGens TestInfo. Import MG.
 Definition forAllEscrowChainBuilder gEscrowTrace length cb := 
   forAllChainBuilder length cb gEscrowTrace .
 
+(* For automation *)
+Instance gEscrowChainBuilder : GenSized ChainBuilder := 
+{|
+  arbitrarySized := gEscrowTraceBetter escrow_chain
+|}.
+Instance shrinkChainBuilder : Shrink ChainBuilder := {| shrink a := [a] |}.
+
 (* Sample (gEscrowMsg escrow_chain). *)
 (* Sample (gEscrowTraceBetter escrow_chain 10). *)
 (* QuickChick (forAll (gEscrowTraceBetter escrow_chain 10) (fun cb =>
@@ -124,6 +131,44 @@ Proof.
   - intros. unfold escrow_correct_Prop. left. rewrite H1 in H0. inversion H0. 
 Qed.
 
+Lemma escrow_correct_bool_false_impl_prop {from to}
+(caddr : Address)
+(cstate : Escrow.State)
+(trace : ChainTrace from to) 
+(depinfo : DeploymentInfo Setup)
+(inc_calls : list (ContractCallInfo Msg)) : 
+  escrow_correct_bool caddr cstate trace depinfo inc_calls = false ->
+  ~(escrow_correct_Prop caddr cstate trace depinfo inc_calls).
+Proof. 
+  unfold escrow_correct_bool.
+  destruct (is_escrow_finished cstate) eqn:H1.
+  - unfold escrow_correct_Prop. 
+    propify. 
+    intros.
+    repeat rewrite Z.eqb_neq in H.
+    intuition.
+  - intros. unfold escrow_correct_Prop. eauto. 
+Qed.
+
+(* Finally, we can show that escrow_correct_Prop is decidable (using escrow_correct_bool as 
+   the decision procedure).  *)
+Instance escrow_correct_P_dec {from to caddr cstate trace depinfo inc_calls} 
+  : Dec (@escrow_correct_Prop from to caddr cstate trace depinfo inc_calls).
+Proof. 
+  constructor. unfold ssrbool.decidable. 
+  destruct (escrow_correct_bool caddr cstate trace depinfo inc_calls) eqn:H.
+  - left. apply escrow_correct_bool_impl_prop. apply H.
+  - right. 
+    unfold not. 
+    intros.
+    apply escrow_correct_bool_false_impl_prop in H.
+    contradiction.
+Defined.
+
+Instance escrow_correct_P_checkable {from to caddr cstate trace depinfo inc_calls}
+  : Checkable (@escrow_correct_Prop from to caddr cstate trace depinfo inc_calls).
+Proof. apply testDec. Defined.
+
 (* Wrapper for escrow_correct_bool. This is the Checker we will run QC on. *)
 Definition escrow_correct_P (cb : ChainBuilder) := 
   let trace := builder_trace cb in
@@ -132,20 +177,26 @@ Definition escrow_correct_P (cb : ChainBuilder) :=
   isSomeCheck depinfo' (fun depinfo =>
     isSomeCheck inc_calls' (fun inc_calls =>
       match get_contract_state Escrow.State cb escrow_contract_addr with
-      | Some cstate => 
-          (escrow_correct_bool escrow_contract_addr cstate trace depinfo inc_calls)
-      | None => false
+      | Some cstate => is_escrow_finished cstate ==>
+        ((escrow_correct_Prop escrow_contract_addr cstate trace depinfo inc_calls)?)
+      | None => checker false
       end
     )
   ).
 
-(* QuickChick (forAllEscrowChainBuilder gEscrowTrace 7 escrow_chain escrow_correct_P). *)
+Extract Constant defNumDiscards => "(3 * defNumTests)".
+
+QuickChick (forAllEscrowChainBuilder gEscrowTrace 7 escrow_chain escrow_correct_P).
 (* *** Gave up! Passed only 8598 tests
 Discarded: 20000 *)
 
 (* Using the better generator, which avoid the discards: *)
 (* QuickChick (forAllEscrowChainBuilder gEscrowTraceBetter 7 escrow_chain escrow_correct_P). *)
 (* +++ Passed 10000 tests (0 discards) *)
+(* Or alternatively we can just write: *)
+(* QuickChick escrow_correct_P. *)
+(* +++ Passed 10000 tests (40 discards) *)
+(* Not sure where the 40 discards come from, but it's an acceptable amount for sure... *)
 
 Definition escrow_next_states {from to} 
                               (escrow_caddr : Address) 
@@ -189,32 +240,148 @@ Definition collect_steps_length_distribution g :=
    buyer_commit -> no_next_step
    Corresponding to the case where the seller withdraws their funds before the buyer commits & confirms their purchase. *)
 
-(* Sample (
-  bindGen (gEscrowTrace escrow_chain 10) (fun cb =>
-    returnGen (escrow_next_states escrow_contract_addr (cb.(builder_trace))))
-). *)
-
-Definition is_valid_step_sequence steps := 
-  let fix rec steps prev_step :=
+Fixpoint is_valid_step_sequence_fix steps prev_step :=
   match prev_step, steps with
   | _, [] => true
-  | None, step::steps' => rec steps' (Some step) 
+  | None, step::steps' => is_valid_step_sequence_fix steps' (Some step) 
   | Some prev_step, step::steps' => match prev_step, step with
                                     | buyer_commit, buyer_confirm
                                     | buyer_commit, no_next_step 
                                     | buyer_confirm, withdrawals
-                                    | withdrawals, no_next_step => rec steps' (Some step)
+                                    | withdrawals, no_next_step => is_valid_step_sequence_fix steps' (Some step)
                                     | _, _ => false
                                     end
-  end in
-  rec steps None.
+  end.
 
-Definition escrow_valid_steps_P cb := 
-  let trace := builder_trace cb in
-  let steps := escrow_next_states escrow_contract_addr trace in
-  is_valid_step_sequence steps.
+Definition is_valid_step_sequence steps := 
+  is_valid_step_sequence_fix steps None.
 
-(* QuickChick (forAllEscrowChainBuilder gEscrowTrace 7 escrow_chain (checker o escrow_valid_steps_P)). *)
+
+Conjecture escrow_valid_steps_P : forall trace : {to : ChainState & ChainTrace empty_state to},
+  let steps := escrow_next_states escrow_contract_addr (projT2 trace) in
+  is_valid_step_sequence steps = true.
+(* Note that we are implicitly using the "better" generator here to generate arbitrary ChainTraces *)
+(* QuickChick escrow_valid_steps_P. *)
 (* +++ Passed 10000 tests (0 discards) *)
- 
 
+Corollary escrow_correct
+            {ChainBuilder : ChainBuilderType}
+            prev new header acts :
+    builder_add_block prev header acts = Ok new ->
+    let trace := builder_trace new in
+    forall caddr,
+      env_contracts new caddr = Some (Escrow.contract : WeakContract) ->
+      let next_states := escrow_next_states caddr trace in
+      is_valid_step_sequence next_states = true.
+Proof.
+Admitted.  (* intros after_add trace caddr escrow_at_caddr next_states. *)
+  (* unfold trace.
+  contract_induction.
+  contract_induction; cbn in *; intros.
+  - (* New block *)
+    auto.
+  - (* Deployment *)
+    unfold Escrow.init in *.
+    destruct (address_eqb_spec (setup_buyer setup) (ctx_from ctx));
+      cbn in *; try congruence.
+    destruct (ctx_amount ctx =? 0) eqn:amount_some; cbn in *; try congruence.
+    destruct (Z.even (ctx_amount ctx)) eqn:amount_even; cbn in *; try congruence.
+    inversion init_some; subst; clear init_some.
+    cbn.
+    assert (2 * (ctx_amount ctx / 2) > 0 -> ctx_amount ctx / 2 > 0) by lia.
+    enough (2 * (ctx_amount ctx / 2) > 0 /\
+            ctx_amount ctx = 2 * (ctx_amount ctx / 2)) by tauto.
+    assert (ctx_amount ctx mod 2 = 0).
+    {
+      rewrite Zeven_mod in amount_even.
+      unfold Zeq_bool in *.
+      destruct_match eqn:amount_mod_2 in amount_even; try congruence; auto.
+      destruct (Z.compare_spec (ctx_amount ctx mod 2) 0); auto; try congruence.
+    }
+    rewrite <- (Z_div_exact_2 (ctx_amount ctx) 2) by (auto; lia).
+    split; auto.
+    instantiate (DeployFacts := fun _ ctx => ctx_amount ctx >= 0);
+      subst DeployFacts; cbn in *.
+    apply Z.eqb_neq in amount_some.
+    lia. *)
+
+(* 
+    intros after_add trace caddr escrow_at_caddr.
+    cbn in *.
+    pose proof (escrow_correct_strong _ caddr trace escrow_at_caddr) as general.
+    cbn in general.
+    destruct general as
+        [cstate [depinfo [inc_calls [? [? [? [? [? [? [? [? [_ IH]]]]]]]]]]]].
+    exists depinfo, cstate, inc_calls.
+    do 3 (split; [tauto|]).
+    intros is_finished.
+    unfold is_escrow_finished in *.
+    destruct (next_step cstate); try congruence; clear is_finished.
+    unfold net_balance_effect, money_to.
+    assert (inc_txs:
+              forall addr,
+                sumZ tx_amount (txs_from addr (incoming_txs trace caddr)) =
+                sumZ (fun '(a, b, c) => c)
+                     (filter (fun '(from, _, _) => (from =? addr)%address)
+                             (map (fun tx => (tx_from tx, tx_to tx, tx_amount tx))
+                                  (incoming_txs trace caddr)))).
+    {
+      intros addr.
+      induction (incoming_txs trace caddr) as [|hd tl IH'].
+      - reflexivity.
+      - rewrite txs_from_cons.
+        cbn.
+        destruct_address_eq; cbn in *; rewrite IH'; reflexivity.
+    }
+
+    repeat rewrite inc_txs; clear inc_txs.
+    rewrite (incoming_txs_contract caddr _ trace _ depinfo _ inc_calls) by assumption.
+    repeat rewrite filter_app, sumZ_app.
+    cbn.
+    rewrite address_eq_refl.
+    rewrite address_eq_ne by auto.
+    cbn.
+    rewrite 2!filter_map, 2!sumZ_map.
+
+    set (buyer_addr := setup_buyer (deployment_setup depinfo)) in *.
+    set (seller_addr := deployment_from depinfo) in *.
+
+    unfold money_to, transfer_acts_to in IH.
+    cbn in IH.
+
+    change (fun a => call_amount a) with (@call_amount _ Msg).
+
+    destruct IH as [IH | IH]; [left|right].
+    - split; [tauto|].
+      remember (build_call_info _ _ (Some commit_money)) as commitment.
+      assert (Hsum :
+                forall f,
+                  sumZ call_amount (filter f inc_calls) =
+                  sumZ call_amount (filter f [commitment])).
+      {
+        intros f.
+        destruct IH as [_ [<- ?]].
+        clear -inc_calls.
+        induction inc_calls as [|hd tl IH']; auto.
+        cbn.
+        destruct (Z.eqb_spec (call_amount hd) 0) as [zero_amount|].
+        - cbn.
+          destruct (f hd); cbn; try rewrite zero_amount; rewrite IH'; auto.
+        - cbn.
+          destruct (f hd); cbn; rewrite IH'; auto.
+      }
+
+      rewrite 2!Hsum; clear Hsum; subst commitment; cbn in *.
+      rewrite address_eq_refl, address_eq_ne by auto.
+      cbn.
+      destruct IH as [_ [_ [? ?]]].
+      split; lia.
+    - destruct IH as [-> IH].
+      cbn.
+      rewrite address_eq_refl, address_eq_ne by auto.
+      cbn.
+      split; [auto|].
+      split; lia.
+  Qed.
+
+*)
